theories/L/Complexity/Cook/FlatPR.v
@@ -14,7 +14,11 @@ Record FlatPR := {
   steps : nat
   }.
 
-Definition PRWin_ofFlatType k (win : PRWin nat) := list_ofFlatType k (prem win) /\ list_ofFlatType k (conc win). 
+Definition PRWin_ofFlatType (win : PRWin nat) k:= list_ofFlatType k (prem win) /\ list_ofFlatType k (conc win). 
+
+Definition isValidFlatWindows (l : list (PRWin nat)) k := (forall win, win el l -> PRWin_ofFlatType win k).
+Definition isValidFlatFinal (l : list (list nat)) k := (forall s, s el l -> list_ofFlatType k s).
+Definition isValidFlatInitial (l : list nat) k := list_ofFlatType k l.
 
 Definition FlatPR_wellformed fpr := 
   width fpr > 0 
@@ -22,12 +26,14 @@ Definition FlatPR_wellformed fpr :=
   /\ (exists k, k > 0 /\ width fpr = k * offset fpr)
   /\ length (init fpr) >= width fpr
   /\ (forall win, win el windows fpr -> PRWin_of_size win (width fpr)) 
-  /\ (exists k, length (init fpr) = k * offset fpr)
-  /\ list_ofFlatType (Sigma fpr) (init fpr) 
-  /\ (forall s, s el final fpr -> list_ofFlatType (Sigma fpr) s)
-  /\ (forall win, win el windows fpr -> PRWin_ofFlatType (Sigma fpr) win). 
+  /\ (exists k, length (init fpr) = k * offset fpr). 
 
-Definition FlatPRLang (C : FlatPR) := FlatPR_wellformed C 
+Definition isValidFlattening fpr := 
+ list_ofFlatType (Sigma fpr) (init fpr) 
+  /\ (forall s, s el final fpr -> list_ofFlatType (Sigma fpr) s)
+  /\ (forall win, win el windows fpr -> PRWin_ofFlatType win (Sigma fpr)). 
+
+Definition FlatPRLang (C : FlatPR) := FlatPR_wellformed C /\ isValidFlattening C
   /\ exists (sf : list nat), list_ofFlatType (Sigma C) sf 
       /\ relpower (valid (offset C) (width C) (windows C)) (steps C) (init C) sf 
       /\ satFinal (offset C) (length (init C)) (final C) sf.
@@ -43,6 +49,7 @@ Section fixInstance.
   Notation steps := (steps fpr). 
 
   Context (A : FlatPR_wellformed fpr). 
+  Context (B : isValidFlattening fpr). 
 
   Lemma app_length_split (X : Type) (v u b c : list X) : v ++ b = u ++ c -> |v| <= |u| -> exists u', u = v ++ u'. 
   Proof. 
@@ -70,7 +77,8 @@ Section fixInstance.
         clear IHvalid H2 l. 
         now eapply G1. 
       + clear IHvalid. clear G1. 
-        destruct A as (_ & _ & (k & _ & A2) & _ & A6 & _ & _ & _ & A5).  
+        destruct A as (_ & _ & (k & _ & A2) & _ & A6 & _).  
+        destruct B as ( _ & _ & A5).
         specialize (A5 _ H5) as (A5 & A7). 
         specialize H6 as ((rest' & H6') & (rest & H6)).  (*show rest = [] *)
         (*we need some structural assumptions *)
@@ -105,12 +113,12 @@ Section fixInstance.
     - intros. apply list_ofFlatType_app. 
     - apply H0. 
     - intros. destruct H2 as (_ & (c & H2)). 
-        destruct A as (_ & _ & A3 & _ & A1 & _ & _ & _ & A2). 
+        destruct A as (_ & _ & A3 & _ & A1 & _ ). destruct B as ( _ & _ & A2).
         specialize (A1 _ H3) as (_ & A1). specialize (A2 _ H3) as (_ & A2). 
         apply app_length_split in H2 as (u' & H2). 
         * rewrite H2 in A2. now apply list_ofFlatType_app in A2. 
         * destruct A3 as (ak & A3 & A4). nia.  
-    - intros. destruct A as (_ & _ & _ & _ & _ & _ & _ & _ & A1). 
+    - intros. destruct B as (_ & _ & A1). 
       apply A1 in H2 as (_ & H2). apply H2. 
     - apply H1. 
   Qed. 
@@ -123,7 +131,72 @@ Section fixInstance.
     - apply H0.  
     - apply valid_length_inv in H1. lia. 
   Qed. 
+
 End fixInstance.
+
+(*deciders for isValidFlattening and well-formedness *)
+Definition ofFlatType_dec (b a : nat) := leb (S a) b.
+Definition list_ofFlatType_dec (t : nat)  (s : list nat) := forallb (ofFlatType_dec t) s. 
+
+Definition PRWin_ofFlatType_dec (Sigma : nat) (win : PRWin nat) := list_ofFlatType_dec Sigma (prem win) && list_ofFlatType_dec Sigma (conc win). 
+
+Lemma leb_iff a b : leb a b = true <-> a <= b. 
+Proof. 
+  split; intros. 
+  - now apply leb_complete. 
+  - now apply leb_correct. 
+Qed.
+
+Lemma list_ofFlatType_dec_correct s t : list_ofFlatType_dec t s = true <-> list_ofFlatType t s. 
+Proof. 
+  unfold list_ofFlatType_dec, list_ofFlatType. rewrite forallb_forall. 
+  unfold ofFlatType_dec. setoid_rewrite leb_iff. 
+  split; intros H; intros; now apply H.
+Qed. 
+
+Lemma PRWin_ofFlatType_dec_correct win Sigma : PRWin_ofFlatType_dec Sigma win = true <-> PRWin_ofFlatType win Sigma. 
+Proof. 
+  unfold PRWin_ofFlatType_dec, PRWin_ofFlatType. rewrite andb_true_iff. 
+  rewrite !list_ofFlatType_dec_correct. easy. 
+Qed. 
+
+Definition FlatPR_wf_dec (fpr : FlatPR) := 
+  leb 1 (width fpr) 
+  && leb 1 (offset fpr)
+  && Nat.eqb (Nat.modulo (width fpr) (offset fpr)) 0
+  && leb (width fpr) (|init fpr|)
+  && forallb (PRWin_of_size_dec (width fpr)) (windows fpr)
+  && Nat.eqb (Nat.modulo (|init fpr|) (offset fpr)) 0. 
+Definition isValidFlattening_dec (fpr : FlatPR) := 
+  list_ofFlatType_dec (Sigma fpr) (init fpr)
+  && forallb (list_ofFlatType_dec (Sigma fpr)) (final fpr)
+  && forallb (PRWin_ofFlatType_dec (Sigma fpr)) (windows fpr). 
+
+Lemma FlatPR_wf_dec_correct (fpr : FlatPR) : FlatPR_wf_dec fpr = true <-> FlatPR_wellformed fpr. 
+Proof. 
+  unfold FlatPR_wf_dec, FlatPR_wellformed. rewrite !andb_true_iff, !and_assoc.
+  rewrite !leb_iff. rewrite <- !(reflect_iff _ _ (Nat.eqb_spec _ _ )).  
+  rewrite !forallb_forall. 
+  setoid_rewrite PRWin_of_size_dec_correct. 
+  split; intros; repeat match goal with [H : _ /\ _ |- _] => destruct H end; 
+  repeat match goal with [ |- _ /\ _ ] => split end; try easy. 
+  - apply Nat.mod_divide in H1 as (k & H1); [ | lia]. 
+    exists k; split; [ | apply H1 ]. destruct k; cbn in *; lia.
+  - apply Nat.mod_divide in H4 as (k & H4); [ | lia].  exists k; apply H4.  
+  - apply Nat.mod_divide; [ lia | ]. destruct H1 as (k & _ & H1). exists k; apply H1.
+  - apply Nat.mod_divide; [ lia | ]. apply H4. 
+Qed. 
+
+Lemma isValidFlattening_dec_correct (fpr : FlatPR) : isValidFlattening_dec fpr = true <-> isValidFlattening fpr. 
+Proof. 
+  unfold isValidFlattening_dec, isValidFlattening.
+  rewrite !andb_true_iff, !and_assoc.
+  rewrite !forallb_forall. 
+  setoid_rewrite PRWin_ofFlatType_dec_correct. 
+  setoid_rewrite list_ofFlatType_dec_correct. 
+  split; intros; repeat match goal with [H : _ /\ _ |- _] => destruct H end; 
+  repeat match goal with [ |- _ /\ _ ] => split end; try easy. 
+Qed. 
 
 (*relation to PR instances *)
 Inductive isFlatPRWinOf (X : finType) (flatwin : PRWin nat) (win : PRWin X) := 
@@ -148,42 +221,280 @@ Inductive isFlatPROf (fpr : FlatPR) (pr : PR) :=
     (HInit : isFlatListOf (init fpr) (PR.init pr))
     (HWindows : isFlatWindowsOf (windows fpr) (PR.windows pr))
     (HFinal : isFlatFinalOf (final fpr) (PR.final pr))
+    (HSteps : steps fpr = PR.steps pr)
   : isFlatPROf fpr pr.
 
+Lemma isFlatPROf_isValidFlattening (fpr : FlatPR) (pr : PR) : isFlatPROf fpr pr -> isValidFlattening fpr. 
+Proof. 
+  intros. destruct H.
+  repeat split.
+  - rewrite HSigma. now eapply isFlatListOf_list_ofFlatType. 
+  - intros s H0%HFinal. rewrite HSigma. destruct H0 as (s' & F1 & ->). 
+    eapply isFlatListOf_list_ofFlatType. unfold isFlatListOf. reflexivity. 
+  - apply HWindows in H. destruct H as (win' & F1 & F2). 
+    destruct F2 as (F2 & F3). rewrite HSigma. 
+    eapply isFlatListOf_list_ofFlatType, F2. 
+  - apply HWindows in H. destruct H as (win' & F1 & F2). 
+    destruct F2 as (F2 & F3). rewrite HSigma. 
+    eapply isFlatListOf_list_ofFlatType, F3. 
+Qed. 
+
+(*we show that FlatPR instances "behave in the same way" as PR instances  *)
+
+(*this is completely similar to the corresponding proof for FlatTPR *)
+Lemma rewritesHead_flat_agree (X : finType) (windowsFin : list (PRWin X)) windowsFlat finStr finStr' flatStr flatStr' :
+  isFlatListOf flatStr finStr
+  -> isFlatListOf flatStr' finStr'
+  -> isFlatWindowsOf windowsFlat windowsFin 
+  -> (exists win, win el windowsFin /\ rewritesHead win finStr finStr') <-> (exists win, win el windowsFlat /\ rewritesHead win flatStr flatStr'). 
+Proof. 
+  intros. split; intros (win & H2 & H3).
+  - apply H1 in H2 as (win' & F1 & F2). exists win'. split; [apply F1 | ]. 
+    unfold rewritesHead, prefix in *. destruct H3 as ((b1 & ->) & (b2 & ->)). 
+    unfold isFlatListOf in H, H0.
+    rewrite map_app in H, H0. split.
+    + exists (map index b1). rewrite H. enough (map index (prem win) = prem win') as H2.
+      { now setoid_rewrite H2. }
+      destruct win; cbn.
+      destruct F2. cbn in *. now rewrite Hprem.  
+    + exists (map index b2). rewrite H0. enough (map index (conc win) = conc win') as H2. 
+      { now setoid_rewrite H2. }
+      destruct win; cbn. 
+      destruct F2. cbn in *. now rewrite Hconc. 
+  - apply H1 in H2 as (win' & F1 & F2). exists win'. split; [ apply F1 | ].
+    unfold rewritesHead, prefix in *. destruct H3 as ((b1 & ->) & (b2 & ->)).
+    unfold isFlatListOf in H, H0. split.
+    + symmetry in H. apply map_eq_app in H as (finStr1  & finStr2 & -> & ? & ?). 
+      exists finStr2.
+      enough (finStr1 = prem win') as H3 by (now setoid_rewrite H3).
+      destruct F2. rewrite Hprem in H. 
+      apply map_injective in H; [easy | unfold injective; apply injective_index]. 
+    + symmetry in H0. apply map_eq_app in H0 as (finStr1  & finStr2 & -> & ? & ?). 
+      exists finStr2.
+      enough (finStr1 = conc win') as H3 by (now setoid_rewrite H3).
+      destruct F2. rewrite Hconc in H0. 
+      apply Prelim.map_inj in H0; [easy | unfold injective; apply injective_index].
+Qed.
+
+Section fixFPRInstance. 
+  Variable (fpr : FlatPR). 
+  Notation Sigma := (Sigma fpr).
+  Notation offset := (offset fpr).
+  Notation width := (width fpr).
+  Notation init := (init fpr).
+  Notation windows := (windows fpr).
+  Notation final := (final fpr).
+  Notation steps := (steps fpr). 
+
+  Context (A : FlatPR_wellformed fpr). 
+  Context (B : isValidFlattening fpr). 
+
+
+  Lemma valid_flat_agree (X : finType) (windows : list (PRWin X)) fwindows s1 s2 fs1 fs2: 
+    isFlatListOf fs1 s1 
+    -> isFlatListOf fs2 s2
+    -> isFlatWindowsOf fwindows windows 
+    -> valid offset width fwindows fs1 fs2 <-> valid offset width windows s1 s2. 
+  Proof. 
+    intros H H1 H2. 
+    split.
+    - intros H3. revert s1 s2 H H1. induction H3; intros. 
+      + destruct s1; [ | now unfold isFlatListOf in H]. 
+        destruct s2; [ | now unfold isFlatListOf in H1].
+        constructor. 
+      + unfold isFlatListOf in H4, H5. 
+        symmetry in H4. apply map_eq_app in H4 as (ls1 & ls2 & -> & -> & ->). 
+        symmetry in H5. apply map_eq_app in H5 as (rs1 & rs2 & -> & -> & ->).
+        constructor 2. 
+        2-4: now rewrite map_length in *. 
+        apply IHvalid; easy. 
+      + unfold isFlatListOf in H5, H6.
+        symmetry in H5. apply map_eq_app in H5 as (ls1 & ls2 & -> & -> & ->). 
+        symmetry in H6. apply map_eq_app in H6 as (rs1 & rs2 & -> & -> & ->).
+        assert (exists w, w el fwindows /\ rewritesHead w (map index ls1 ++ map index ls2) (map index rs1 ++ map index rs2)) as H5 by eauto.
+        eapply rewritesHead_flat_agree in H5 as (finwin & H5 & H6). 
+        * econstructor 3. 2-3: now rewrite map_length in *. 
+          -- eapply IHvalid; easy.
+          -- apply H5. 
+          -- apply H6. 
+        * clear H5 H6. apply isFlatListOf_app; easy.
+        * clear H5 H6. apply isFlatListOf_app; easy.
+        * clear H5 H6. apply H2. 
+    - intros H3. revert fs1 fs2 H H1 H2. induction H3; intros.
+      + rewrite H, H1; cbn; constructor 1.  
+      + rewrite H2, H4. rewrite !map_app. constructor. 2-4: rewrite map_length; auto.
+        now eapply IHvalid.
+      + rewrite H4, H5. rewrite !map_app. 
+        assert (exists w, w el windows /\ rewritesHead w (u ++ a) (v++b)) as H7 by eauto.
+        eapply rewritesHead_flat_agree in H7 as (finwin & H7 & H8). 2-4: eauto.
+        econstructor 3. 2-3: rewrite map_length; auto.
+        * now eapply IHvalid.
+        * apply H7. 
+        * rewrite H4, H5 in H8. now rewrite !map_app in H8. 
+  Qed. 
+
+  (*we re-use the lemma proven above which asserts that list_ofFlatType is invariant *)
+  (*for that, we need more assumptions than are required in principle, but this is okay *)
+  Lemma valid_flat_isFlatListOf_invariant (X : finType) (s1 : list X) fs1 fs2: 
+    finRepr X Sigma
+    -> isFlatListOf fs1 s1
+    -> |fs1| >= width 
+    -> valid offset width windows fs1 fs2
+    -> exists (s2 : list X), isFlatListOf fs2 s2. 
+  Proof. 
+    intros. 
+    apply isFlatListOf_list_ofFlatType in H0. rewrite <- H in H0. 
+    specialize (@valid_list_ofFlatType_invariant fpr A B fs1 fs2 H0 H1 H2) as H4. 
+    apply (finRepr_exists_list H) in H4. destruct H4 as (s2 & H4); easy.
+  Qed. 
+
+  Lemma relpower_valid_flat_agree (X : finType) (finwindows : list (PRWin X)) s1 s2 fs1 fs2 n:
+    finRepr X Sigma
+    -> |fs1| >= width 
+    -> isFlatListOf fs1 s1
+    -> isFlatListOf fs2 s2
+    -> isFlatWindowsOf windows finwindows
+    -> relpower (valid offset width windows) n fs1 fs2 <-> relpower (valid offset width finwindows) n s1 s2.
+  Proof. 
+    intros H0 H1 H2 H3 H4. split.
+    - intros H5. revert s1 s2 H2 H3. induction H5; intros. 
+      + specialize (isFlatListOf_functional H2 H3) as ->. eauto.
+      + specialize (valid_flat_isFlatListOf_invariant H0 H2 H1 H) as (s3 & H6).  
+        specialize (valid_length_inv H) as H7. rewrite H7 in H1. 
+        specialize (IHrelpower H1  _ _ H6 H3). 
+        econstructor. 
+        * apply (valid_flat_agree H2 H6 H4) in H. apply H. 
+        * apply IHrelpower. 
+    - intros H5. clear H1. 
+      revert fs1 fs2 H2 H3. induction H5; intros. 
+      + specialize (isFlatListOf_injective H2 H3) as ->. constructor. 
+      + assert (isFlatListOf (map index b) b) as H1 by (unfold isFlatListOf; easy).
+        specialize (IHrelpower _ _ H1 H3). 
+        apply (valid_flat_agree H2 H1 H4) in H. eauto. 
+  Qed. 
+
+  Lemma final_flat_agree (X : finType) (F : list (list X)) (f : list (list nat)) l: 
+    isFlatFinalOf f F -> forall s fs, isFlatListOf fs s -> satFinal offset l f fs <-> satFinal offset l F s. 
+  Proof. 
+    intros. split. 
+    - intros (subs & k & H1 & H2 & H3). apply H in H1 as (subs' & H4 & H5). 
+      exists subs', k. split; [ apply H4 | split; [ apply H2 | ]]. 
+      unfold isFlatListOf in H0. rewrite H0 in H3. rewrite H5 in H3.  
+      destruct H3 as (b & H3). rewrite <- utils.map_skipn in H3. 
+      apply map_eq_app in H3 as (ls1 & ls2 & H3 & H6 & H7). 
+      rewrite H3. 
+      apply map_injective in H6; [ | apply injective_index]. 
+      rewrite H6. now exists ls2.
+    - intros (subs & k & H1 & H2 & H3). apply H in H1 as (subs' & H4 &H5). 
+      exists subs', k. split; [ apply H4 | split; [ apply H2 | ]]. 
+      rewrite H5, H0. destruct H3 as (b & H3). 
+      exists (map index b). rewrite <- utils.map_skipn. rewrite H3. 
+      now rewrite !map_app.
+  Qed. 
+End fixFPRInstance. 
+
+Lemma isFlatPROf_wf_equivalent (pr : PR) (fpr : FlatPR) : 
+  isFlatPROf fpr pr -> (FlatPR_wellformed fpr <-> PR_wellformed pr). 
+Proof. 
+  intros [H1 H2 H3 H4]. split; intros; unfold FlatPR_wellformed, PR_wellformed in *.
+  - destruct H as (F1 & F2 & F3 & F4 & F5 & F6). repeat split.  
+    + easy.
+    + easy.
+    + destruct F3 as (k & F3 & F3'). exists k. nia.
+    + rewrite -> H4 in F4. rewrite map_length in F4. lia. 
+    + apply HWindows in H as (flatwin & H & H5). apply F5 in H. 
+      destruct H5. destruct H as (H & _). rewrite Hprem in H. rewrite map_length in H. lia.  
+    + apply HWindows in H as (flatwin & H & H5). apply F5 in H. 
+      destruct H5. destruct H as (_ & H). rewrite Hconc in H. rewrite map_length in H. lia.  
+    + destruct F6 as (k & F6). rewrite H4 in F6. rewrite map_length in F6. exists k; nia.
+  - destruct H as (F1 & F2 & F3 & F4 & F5 & F6). repeat split. 
+    + easy. 
+    + easy. 
+    + destruct F3 as (k & F3 & F3'). exists k. nia. 
+    + rewrite H4, map_length. lia.  
+    + apply HWindows in H as (finwin & H & H5). apply F5 in H. 
+      destruct H5. destruct H as (H & _). rewrite Hprem, map_length. lia.  
+    + apply HWindows in H as (finwin & H & H5). apply F5 in H. 
+      destruct H5. destruct H as (_ & H). rewrite Hconc, map_length. lia. 
+    + destruct F6 as (k & F6). rewrite H4, map_length. exists k. nia. 
+Qed. 
+
+Lemma isFlatPROf_equivalence (pr : PR) (fpr : FlatPR) : 
+  isFlatPROf fpr pr -> (FlatPRLang fpr <-> PRLang pr). 
+Proof. 
+  intros. split. 
+  - intros (H1 & H2 & H3). split; [ now eapply isFlatPROf_wf_equivalent | ]. 
+    destruct H as [F1 F2 F3 F4 F5].
+    destruct H3 as (sf & H3 & H4 & H5).
+    apply (finRepr_exists_list F1) in H3 as (SF & H3).
+    exists SF. split. 
+    + rewrite <- F2, <- F3, <- HSteps. eapply relpower_valid_flat_agree; eauto. apply H1.    
+    + rewrite <- F2. rewrite F4, map_length in H5. eapply final_flat_agree; eauto.
+  - intros (H1 & H2). split; [ now eapply isFlatPROf_wf_equivalent | ]. 
+    split; [now eapply isFlatPROf_isValidFlattening | ].
+    destruct H as [F1 F2 F3 F4 F5]. 
+    destruct H2 as (sf & H3 & H4). 
+    exists (map index sf). repeat split. 
+    + unfold list_ofFlatType, ofFlatType. 
+      setoid_rewrite in_map_iff. intros a (x & <- & H). rewrite F1. apply index_le. 
+    + eapply relpower_valid_flat_agree; eauto.
+      * now rewrite isFlatPROf_wf_equivalent. 
+      * now eapply isFlatPROf_isValidFlattening with (pr := pr). 
+      * rewrite F4, map_length, F3. apply H1. 
+      * unfold isFlatListOf. reflexivity. 
+      * rewrite  F2,  F3, HSteps. apply H3. 
+    + eapply final_flat_agree; eauto. 
+      * unfold isFlatListOf; reflexivity. 
+      * rewrite F2, F4, map_length. apply H4. 
+Qed. 
+
 (*given a well-formed flat instance, we can derive a "canonical" (up to bijections of the finite type) PR instance *)
+(*unflattening *)
+Require Import PslBase.FiniteTypes.VectorFin PslBase.FiniteTypes.Cardinality. 
+Lemma unflattenString (f : list nat) k : list_ofFlatType k f -> sigT (fun (f' : list (finType_CS (Fin.t k))) => isFlatListOf f f'). 
+Proof. 
+  intros H. 
+  eapply finRepr_exists_list with (X := finType_CS (Fin.t k)) in H as (a' & H). 
+  2: { unfold finRepr. specialize (Card_Fint k). unfold Cardinality. easy. }
+  eauto.
+Qed. 
 
-(*Section fixFlat. *)
-  (*Variable (fpr : FlatPR). *)
-  (*Context (A : FlatPR_wellformed fpr). *)
+Lemma unflattenWindow (w : PRWin nat) k : PRWin_ofFlatType w k -> sigT (fun (w' : PRWin (finType_CS (Fin.t k))) => isFlatPRWinOf w w'). 
+Proof. 
+  intros. destruct w. destruct H as (H1 & H2). cbn in *.
+  apply unflattenString in H1 as (prem' & H1). 
+  apply unflattenString in H2 as (conc' & H2).
+  exists (Build_PRWin prem' conc'). split; easy.
+Qed. 
 
-  (*Definition FSigma := Fin.t (Sigma fpr). *)
-  (*Definition Foffset := offset fpr. *)
-  (*Definition Fwidth := width fpr. *)
-  (*Definition Fsteps := steps fpr. *)
+Lemma unflattenWindows (l : list (PRWin nat)) k : isValidFlatWindows l k -> sigT (fun (l' : list (PRWin (finType_CS (Fin.t k)))) => isFlatWindowsOf l l').  
+Proof. 
+  intros. unfold isValidFlatWindows in H. induction l. 
+  - exists []. easy.
+  - edestruct IHl as (l' & IH);[ easy | ]. specialize (H a (or_introl eq_refl)). 
+    apply unflattenWindow in H as (a' & H). exists (a' :: l'). split; intros.
+    + destruct H0 as [-> | H0]; [easy | ]. apply IH in H0 as (win & ? & ?); eauto.
+    + destruct H0 as [-> | H0]; [ easy | ]. apply IH in H0 as (win' & ? & ?); eauto.
+Qed. 
 
-  (*Lemma list_ofFlatType_cons x y k : list_ofFlatType k (x :: y) <-> ofFlatType k x /\ list_ofFlatType k y. *)
-  (*Proof. *)
-    (*split; unfold list_ofFlatType; intros. *)
-    (*- split; [ apply H; eauto | intros; apply H; eauto]. *)
-    (*- destruct H0 as [-> | H0]. *)
-      (*+ apply (proj1 H). *)
-      (*+ apply (proj2 H), H0. *)
-  (*Qed. *)
+Lemma unflattenFinal (f : list (list nat)) k : isValidFlatFinal f k -> sigT (fun (f' : list (list (finType_CS (Fin.t k)))) => isFlatFinalOf f f'). 
+Proof. 
+  intros. unfold isValidFlatFinal in H. induction f; intros.
+  - exists []; easy.
+  - edestruct IHf as (f' & IH); [easy | ]. specialize (H a (or_introl eq_refl)). 
+    apply unflattenString in H as (a' &H).
+    exists (a'::f'). split; intros. 
+    + destruct H0 as [-> | H0]; [easy | ]. apply IH in H0 as (? & ? & ?); eauto.
+    + destruct H0 as [-> | H0]; [easy | ]. apply IH in H0 as (? & ? & ?); eauto.
+Qed. 
 
-  (*Lemma index_of_nat n k (H : k < n) : index (Fin.of_nat_lt H) = k. *)
-  (*Proof. *)
-    (*induction k. *)
-    (*- cbn. destruct n; cbn; [ exfalso; lia | ]. unfold index. cbn. destruct False_rect; cbn. unfold False_rect. Check Nat.nlt_0_r. *)
-
-  (*Lemma Fstring (x : list nat) : list_ofFlatType (Sigma fpr) x -> {y : list FSigma & isFlatListOf x y}. *)
-  (*Proof. *)
-    (*intros. induction x. *)
-    (*- exists []. unfold isFlatListOf. easy. *)
-    (*- apply list_ofFlatType_cons in H as (H & H0). *)
-      (*apply IHx in H0 as (y & H0). exists (Fin.of_nat_lt H :: y). *)
-      (*unfold isFlatListOf. cbn. unfold Fin.of_nat_lt. *)
-      
-      (*SearchAbout list_ofFlatType. *)
-      (*unfold list_ofFlatType *)
-
-  (*Definition Finit := *)
+Lemma unflattenPR (f : FlatPR) : isValidFlattening f -> sigT (fun (f' : PR) => isFlatPROf f f'). 
+Proof. 
+  intros (H1 & H2 & H3).
+  apply unflattenWindows in H3 as (w' & H3). 
+  apply unflattenFinal in H2 as (f' & H2). 
+  apply unflattenString in H1 as (i' & H1). 
+  exists (Build_PR (offset f) (width f) i' w' f' (steps f)). 
+  constructor; eauto.
+  cbn. unfold finRepr. specialize (Card_Fint (Sigma f)). easy.  
+Qed.
