theories/L/Complexity/Cook/FlatPR_to_BinaryPR.v
@@ -1,10 +1,10 @@
 From PslBase Require Import Base. 
 From PslBase Require Import Vectors.Vectors. 
-From Undecidability.L.Complexity.Cook Require Import Prelim BinaryPR FlatPR FlatPR_homomorphisms. 
-From Undecidability.L.Complexity.Cook Require Import FlatPR.
+From Undecidability.L.Complexity.Cook Require Import Prelim UniformHomomorphisms BinaryPR FlatPR PR_to_BinaryPR. 
 Require Import Lia.
 
-Section fixInstance. 
+(*we basically reduce to PR and use the established reduction PR -> BinaryPR *)
+Section fixInstanceA. 
   Variable (fpr : FlatPR). 
 
   Notation Sigma := (Sigma fpr).
@@ -17,134 +17,92 @@ Section fixInstance.
 
   (*we first do the reduction for wellformed instances, satisfying the syntactic requirements *)
   Context (A : FlatPR_wellformed fpr). 
+  Context (B : isValidFlattening fpr). 
   Context (A1 : Sigma > 0). (*instances without this property are trivial no instances *)
-  
-  Definition h' (x : nat) := if leb (S x) Sigma then repEl x false ++ [true] ++ repEl (Sigma - x -1) false
-                                                else repEl Sigma false. 
 
-  Lemma h'_length (x : nat) : |h' x| = Sigma. 
+  (*we use the hNat homomorphism from the PR reduction *)
+  Definition hflat := canonicalHom (hNat Sigma).
+
+  Definition hoffset := Sigma * offset. 
+  Definition hwidth := Sigma * width. 
+  Definition hinit := hflat init.
+  Definition hwindow win := match win with Build_PRWin prem conc => Build_PRWin (hflat prem) (hflat conc) end.
+  Definition hwindows := map hwindow windows. 
+  Definition hfinal := map hflat final. 
+  Definition hsteps := steps. 
+
+  Definition hBinaryPR := @BinaryPR.Build_BinaryPR hoffset hwidth hinit hwindows hfinal hsteps. 
+
+  (*We show that if fpr is the flattening of a PR instance pr, then the produced BinaryPR instances are equivalent *)
+  (*up to reordering of windows and final strings *)
+
+  Variable (pr : PR). 
+  Variable (isFlattening : isFlatPROf fpr pr). 
+
+  Definition finhBinaryPR := PR_to_BinaryPR.hBinaryPR pr.
+
+  Lemma isFlatListOf_hom_agree l L : isFlatListOf l L -> hflat l = @h pr L.  
   Proof. 
-    unfold h'. destruct leb eqn:H. 
-    - rewrite !app_length, !repEl_length. apply leb_complete in H. cbn. nia. 
-    - now rewrite repEl_length.
+    destruct isFlattening. 
+    intros. rewrite H. unfold h, PR_homomorphisms.h. 
+    unfold h', hflat. rewrite <- HSigma. 
+    unfold canonicalHom. now rewrite map_map. 
   Qed. 
 
-  Lemma repEl_app_inv (X : Type) (a : X) s1 s2 n : repEl n a = s1 ++ s2 -> exists n1 n2, s1 = repEl n1 a /\ s2 = repEl n2 a /\ n1 + n2 = n. 
+  Lemma isFlatPRWinOf_hom_agree w W : isFlatPRWinOf w W -> hwindow w = PR_homomorphisms.hwindow (@h' pr) W.
   Proof. 
-    revert s1 s2.  induction n. 
-    - cbn. destruct s1, s2; cbn; try congruence. intros _. exists 0, 0; now cbn.  
-    - cbn. destruct s1. 
-      + cbn. destruct s2; cbn; [ congruence | ]. 
-        intros H. inv H. exists 0, (S n); now cbn. 
-      + intros. cbn in H. inv H. apply IHn in H2 as (n1 & n2 & -> & -> & <-). 
-        exists (S n1), n2; now cbn. 
+    intros. destruct w, W. cbn. 
+    erewrite isFlatListOf_hom_agree; [ | apply H]. 
+    erewrite isFlatListOf_hom_agree; [ | apply H]. 
+    easy.
   Qed. 
 
-  Lemma h'_inv1 (x n : nat) : h' x = repEl n false ++ [true] ++ repEl (Sigma - n -1) false -> x = n. 
+  Lemma isFlatWindowsOf_hom_agree: hwindows === PR_homomorphisms.hwindows (@h' pr).  
   Proof. 
-    intros. unfold h' in H. 
-    destruct leb eqn:H1. 
-    - clear H1. revert H.  generalize (Sigma - x- 1). generalize (Sigma - n -1). 
-      revert n. induction x; intros. 
-      + destruct n; cbn in H; [reflexivity | congruence]. 
-      + destruct n; cbn in H; [ congruence | ]. inv H. now apply IHx in H1.
-    - destruct (le_lt_dec n Sigma). 
-      + assert (|repEl n false| <= |repEl Sigma false|) by (now rewrite !repEl_length). 
-        apply list_length_split1 in H0 as (s1 & s2 & H0 & _ & H2). rewrite H2 in H. 
-        apply app_eq_length in H as (_ & H); [ | apply H0]. 
-        apply repEl_app_inv in H2 as (n1 & n2 & -> & -> & H2).   
-        destruct n2; cbn in H; congruence. 
-      + match type of H with ?a = ?b => assert (|a| = |b|) by congruence end. 
-        rewrite !app_length, !repEl_length in H0. cbn in H0. lia. 
+    split; intros a H;
+    [unfold hwindows in H | unfold PR_homomorphisms.hwindows in H]; apply in_map_iff in H as (win & <- & H); apply isFlattening in H as (win' & H & H1); 
+      apply isFlatPRWinOf_hom_agree in H1; apply in_map_iff; eauto.  
   Qed. 
 
-  Definition h (x : list nat) := concat (map h' x). 
-
-  Lemma h_uniform_homomorphism : uniform_homomorphism h. 
+  Lemma isFlatFinalOf_hom_agree: hfinal === PR_homomorphisms.hfinal (@h' pr).
   Proof. 
-    split; [ | split].
-    + unfold homomorphism. intros. unfold h. now rewrite map_app, concat_app. 
-    + intros. unfold h. cbn. rewrite !app_nil_r. now rewrite !h'_length. 
-    + intros. cbn. rewrite app_length, h'_length. cbn. lia. 
+    split; intros a H; [unfold hfinal in H | unfold PR_homomorphisms.hfinal in H]; 
+    apply in_map_iff in H as (subs & <- & H); apply isFlattening in H as (subs' & H & H1);
+      apply isFlatListOf_hom_agree in H1; apply in_map_iff; eauto. 
   Qed. 
 
-  Lemma h_bounded_injective : bounded_injectivity Sigma (hsingle h). 
+  Lemma BinaryPR_instances_wf_equivalent : BinaryPR_wellformed finhBinaryPR <-> BinaryPR_wellformed hBinaryPR. 
   Proof. 
-    unfold bounded_injectivity. intros. 
-    unfold hsingle in H0. cbn in H0. rewrite !app_nil_r in H0. 
-    symmetry in H0. unfold h' in H0. erewrite (leb_correct (S n1)) in H0.  
-    - now apply h'_inv1 in H0. 
-    - lia. 
+    destruct isFlattening. 
+    unfold BinaryPR_wellformed. cbn. unfold PR_homomorphisms.hwidth, PR_homomorphisms.hoffset, hwidth, hoffset.  
+    rewrite <- !HSigma, <- !HWidth, <- !HOffset. 
+    split; intros (H1 & H2 & H3 & H4 &H5 & H6); repeat match goal with [ |- _ /\ _] => split end; try easy.
+    - unfold hinit. erewrite isFlatListOf_hom_agree; [ | easy]. apply H4. 
+    - intros. rewrite (isFlatWindowsOf_hom_agree) in H. easy.
+    - unfold hinit. erewrite isFlatListOf_hom_agree; [ | easy]. apply H6. 
+    - unfold hinit in H4. erewrite isFlatListOf_hom_agree in H4; [ | easy]. apply H4. 
+    - intros. rewrite <- (isFlatWindowsOf_hom_agree) in H. easy.
+    - unfold hinit in H6. erewrite isFlatListOf_hom_agree in H6; [ | easy]. apply H6. 
   Qed. 
 
-  (*we now get the reduction for the case that the instance we reduce from is wellformed *)
-  Lemma reduction_wf : FlatPRLang fpr <-> BinaryPRLang (hBinaryPR h fpr). 
+  Lemma BinaryPR_instances_equivalent : BinaryPRLang finhBinaryPR <-> BinaryPRLang hBinaryPR. 
   Proof. 
-    specialize (h_bounded_injective) as F1. 
-    specialize (h_uniform_homomorphism) as F2. 
-    split; intros. 
-    - destruct H as (_ & sf & H1 & H2 & H3).
-      split; [ apply FlatPR_homomorphism_wf; auto | ]. 
-      apply FlatPR_homomorphism_iff; eauto. 
-    - destruct H as (_ & H1).
-      split; [ apply A | ]. 
-      apply FlatPR_homomorphism_iff in H1; eauto. 
+    unfold BinaryPRLang. destruct isFlattening. 
+    cbn. unfold PR_homomorphisms.hwidth, PR_homomorphisms.hoffset, hwidth, hoffset, PR_homomorphisms.hsteps, hsteps.  
+    rewrite <- !HSigma, <- !HWidth, <- !HOffset, <- !HSteps. 
+    unfold hinit, PR_homomorphisms.hinit. setoid_rewrite isFlatListOf_hom_agree; [ | easy | easy].
+
+    split; intros (Hwf & sf & H1 & H2 );
+    (split; [ apply BinaryPR_instances_wf_equivalent, Hwf| exists sf; split ]).
+    - eapply relpower_congruent. 2: apply H1. intros. eapply valid_windows_equivalent. 
+      apply isFlatWindowsOf_hom_agree.
+    - eapply satFinal_final_equivalent. 2: apply H2. apply isFlatFinalOf_hom_agree. 
+    - eapply relpower_congruent. 2: apply H1. intros. eapply valid_windows_equivalent. 
+      symmetry. apply isFlatWindowsOf_hom_agree.
+    - eapply satFinal_final_equivalent. 2: apply H2. symmetry. apply isFlatFinalOf_hom_agree. 
   Qed. 
-End fixInstance. 
+End fixInstanceA.
 
-Definition ofFlatType_dec (b a : nat) := leb (S a) b.
-Definition list_ofFlatType_dec (t : nat)  (s : list nat) := forallb (ofFlatType_dec t) s. 
-
-Definition PRWin_ofFlatType_dec (Sigma : nat) (win : PRWin nat) := list_ofFlatType_dec Sigma (prem win) && list_ofFlatType_dec Sigma (conc win). 
-
-Lemma leb_iff a b : leb a b = true <-> a <= b. 
-Proof. 
-  split; intros. 
-  - now apply leb_complete. 
-  - now apply leb_correct. 
-Qed.
-
-Lemma list_ofFlatType_dec_correct s t : list_ofFlatType_dec t s = true <-> list_ofFlatType t s. 
-Proof. 
-  unfold list_ofFlatType_dec, list_ofFlatType. rewrite forallb_forall. 
-  unfold ofFlatType_dec. setoid_rewrite leb_iff. 
-  split; intros H; intros; now apply H.
-Qed. 
-
-Lemma PRWin_ofFlatType_dec_correct win Sigma : PRWin_ofFlatType_dec Sigma win = true <-> PRWin_ofFlatType Sigma win. 
-Proof. 
-  unfold PRWin_ofFlatType_dec, PRWin_ofFlatType. rewrite andb_true_iff. 
-  rewrite !list_ofFlatType_dec_correct. easy. 
-Qed. 
-
-
-Definition FlatPR_wf_dec (fpr : FlatPR) := 
-  leb 1 (width fpr) 
-  && leb 1 (offset fpr)
-  && Nat.eqb (Nat.modulo (width fpr) (offset fpr)) 0
-  && leb (width fpr) (|init fpr|)
-  && forallb (PRWin_of_size_dec (width fpr)) (windows fpr)
-  && Nat.eqb (Nat.modulo (|init fpr|) (offset fpr)) 0
-  && list_ofFlatType_dec (Sigma fpr) (init fpr)
-  && forallb (list_ofFlatType_dec (Sigma fpr)) (final fpr)
-  && forallb (PRWin_ofFlatType_dec (Sigma fpr)) (windows fpr). 
-
-Lemma FlatPR_wf_dec_correct (fpr : FlatPR) : FlatPR_wf_dec fpr = true <-> FlatPR_wellformed fpr. 
-Proof. 
-  unfold FlatPR_wf_dec, FlatPR_wellformed. rewrite !andb_true_iff, !and_assoc.
-  rewrite !leb_iff. rewrite <- !(reflect_iff _ _ (Nat.eqb_spec _ _ )).  
-  rewrite !forallb_forall. 
-  setoid_rewrite PRWin_ofFlatType_dec_correct. 
-  setoid_rewrite list_ofFlatType_dec_correct. 
-  setoid_rewrite PRWin_of_size_dec_correct. 
-  split; intros; repeat match goal with [H : _ /\ _ |- _] => destruct H end; 
-  repeat match goal with [ |- _ /\ _ ] => split end; try easy. 
-  - apply Nat.mod_divide in H1 as (k & H1); [ | lia]. 
-    exists k; split; [ | apply H1 ]. destruct k; cbn in *; lia.
-  - apply Nat.mod_divide in H4 as (k & H4); [ | lia].  exists k; apply H4.  
-  - apply Nat.mod_divide; [ lia | ]. destruct H1 as (k & _ & H1). exists k; apply H1.
-  - apply Nat.mod_divide; [ lia | ]. apply H4. 
-Qed. 
 
 Definition trivialNoInstance := Build_BinaryPR 0 0 [] [] [] 0. 
 Lemma trivialNoInstance_isNoInstance : not (BinaryPRLang trivialNoInstance). 
@@ -152,13 +110,137 @@ Proof.
   intros (H & _). destruct H as (H & _). cbn in H. lia. 
 Qed. 
 
-Definition reduction (fpr : FlatPR) := if FlatPR_wf_dec fpr && leb 1 (Sigma fpr) then hBinaryPR (h fpr) fpr else trivialNoInstance. 
+Definition reduction (fpr : FlatPR) := if FlatPR_wf_dec fpr && isValidFlattening_dec fpr then hBinaryPR fpr else trivialNoInstance. 
 
-Lemma reduction_correct (fpr : FlatPR) : FlatPRLang fpr <-> BinaryPRLang (reduction fpr).  
+Lemma FlatPR_to_BinaryPR (fpr : FlatPR) : FlatPRLang fpr <-> BinaryPRLang (reduction fpr).  
 Proof. 
-  (*split; intros (H & H1). *)
-  (*- unfold reduction. rewrite (proj2 (FlatPR_wf_dec_correct _) H). *)
-    (*destruct (lt_dec 0 (Sigma fpr)). *)
-    (*+ *)
-    (*apply reduction_wf. *)
-Admitted. 
+  split; intros. 
+  - destruct H as (H1 & Hwf & H2). 
+    unfold reduction. 
+    rewrite (proj2 (FlatPR_wf_dec_correct _) H1). 
+    rewrite (proj2 (isValidFlattening_dec_correct _) Hwf). 
+    specialize (unflattenPR Hwf) as (pr & H3).
+    eapply BinaryPR_instances_equivalent; [ apply H3 | ]. 
+    apply isFlatPROf_equivalence in H3. 
+    enough (PRLang pr). 
+    { specialize (PR_to_BinaryPR pr) as H4. unfold PR_to_BinaryPR.reduction in H4. 
+      enough (PR_wf_dec pr = true) as H5 by (rewrite H5 in H4; apply H4, H). 
+      destruct H as (H & _ & _). apply PR_wf_dec_correct, H.  
+    } 
+    apply H3; easy.
+  - unfold reduction in H. destruct (FlatPR_wf_dec) eqn:H1, (isValidFlattening_dec) eqn:H2. 
+    2-4: cbn in H; now apply trivialNoInstance_isNoInstance in H.
+    cbn in H. apply isValidFlattening_dec_correct in H2. apply FlatPR_wf_dec_correct in H1. 
+    (*we restore an unflattened instance *)
+    specialize (unflattenPR H2) as (pr & H3). eapply isFlatPROf_equivalence; [ apply H3 | ]. 
+    apply PR_to_BinaryPR. unfold PR_to_BinaryPR.reduction. 
+    enough (PR_wf_dec pr = true) as -> by now eapply BinaryPR_instances_equivalent. 
+    eapply PR_wf_dec_correct, isFlatPROf_wf_equivalent; easy.
+Qed.
+
+(*Section fixInstance. *)
+  (*Variable (fpr : FlatPR). *)
+
+  (*Notation Sigma := (Sigma fpr).*)
+  (*Notation offset := (offset fpr).*)
+  (*Notation width := (width fpr).*)
+  (*Notation init := (init fpr).*)
+  (*Notation windows := (windows fpr).*)
+  (*Notation final := (final fpr).*)
+  (*Notation steps := (steps fpr). *)
+
+  (*[>we first do the reduction for wellformed instances, satisfying the syntactic requirements <]*)
+  (*Context (A : FlatPR_wellformed fpr). *)
+  (*Context (B : isValidFlattening fpr). *)
+  (*Context (A1 : Sigma > 0). [>instances without this property are trivial no instances <]*)
+  
+  (*Definition h' (x : nat) := if leb (S x) Sigma then repEl x false ++ [true] ++ repEl (Sigma - x -1) false*)
+                                                (*else repEl Sigma false. *)
+
+  (*Lemma h'_length (x : nat) : |h' x| = Sigma. *)
+  (*Proof. *)
+    (*unfold h'. destruct leb eqn:H. *)
+    (*- rewrite !app_length, !repEl_length. apply leb_complete in H. cbn. nia. *)
+    (*- now rewrite repEl_length.*)
+  (*Qed. *)
+
+  (*Lemma repEl_app_inv (X : Type) (a : X) s1 s2 n : repEl n a = s1 ++ s2 -> exists n1 n2, s1 = repEl n1 a /\ s2 = repEl n2 a /\ n1 + n2 = n. *)
+  (*Proof. *)
+    (*revert s1 s2.  induction n. *)
+    (*- cbn. destruct s1, s2; cbn; try congruence. intros _. exists 0, 0; now cbn.  *)
+    (*- cbn. destruct s1. *)
+      (*+ cbn. destruct s2; cbn; [ congruence | ]. *)
+        (*intros H. inv H. exists 0, (S n); now cbn. *)
+      (*+ intros. cbn in H. inv H. apply IHn in H2 as (n1 & n2 & -> & -> & <-). *)
+        (*exists (S n1), n2; now cbn. *)
+  (*Qed. *)
+
+  (*Lemma h'_inv1 (x n : nat) : h' x = repEl n false ++ [true] ++ repEl (Sigma - n -1) false -> x = n. *)
+  (*Proof. *)
+    (*intros. unfold h' in H. *)
+    (*destruct leb eqn:H1. *)
+    (*- clear H1. revert H.  generalize (Sigma - x- 1). generalize (Sigma - n -1). *)
+      (*revert n. induction x; intros. *)
+      (*+ destruct n; cbn in H; [reflexivity | congruence]. *)
+      (*+ destruct n; cbn in H; [ congruence | ]. inv H. now apply IHx in H1.*)
+    (*- destruct (le_lt_dec n Sigma). *)
+      (*+ assert (|repEl n false| <= |repEl Sigma false|) by (now rewrite !repEl_length). *)
+        (*apply list_length_split1 in H0 as (s1 & s2 & H0 & _ & H2). rewrite H2 in H. *)
+        (*apply app_eq_length in H as (_ & H); [ | apply H0]. *)
+        (*apply repEl_app_inv in H2 as (n1 & n2 & -> & -> & H2).   *)
+        (*destruct n2; cbn in H; congruence. *)
+      (*+ match type of H with ?a = ?b => assert (|a| = |b|) by congruence end. *)
+        (*rewrite !app_length, !repEl_length in H0. cbn in H0. lia. *)
+  (*Qed. *)
+
+  (*Definition h (x : list nat) := concat (map h' x). *)
+
+  (*Lemma h_uniform_homomorphism : uniform_homomorphism h. *)
+  (*Proof. *)
+    (*split; [ | split].*)
+    (*+ unfold homomorphism. intros. unfold h. now rewrite map_app, concat_app. *)
+    (*+ intros. unfold h. cbn. rewrite !app_nil_r. now rewrite !h'_length. *)
+    (*+ intros. cbn. rewrite app_length, h'_length. cbn. lia. *)
+  (*Qed. *)
+
+  (*Lemma h_bounded_injective : bounded_injectivity Sigma (hsingle h). *)
+  (*Proof. *)
+    (*unfold bounded_injectivity. intros. *)
+    (*unfold hsingle in H0. cbn in H0. rewrite !app_nil_r in H0. *)
+    (*symmetry in H0. unfold h' in H0. erewrite (leb_correct (S n1)) in H0.  *)
+    (*- now apply h'_inv1 in H0. *)
+    (*- lia. *)
+  (*Qed. *)
+
+  (*[>we now get the reduction for the case that the instance we reduce from is wellformed <]*)
+  (*Lemma reduction_wf : FlatPRLang fpr <-> BinaryPRLang (hBinaryPR h fpr). *)
+  (*Proof. *)
+    (*specialize (h_bounded_injective) as F1. *)
+    (*specialize (h_uniform_homomorphism) as F2. *)
+    (*split; intros. *)
+    (*- destruct H as (_ & sf & H1 & H2 & H3).*)
+      (*split; [ apply FlatPR_homomorphism_wf; auto | ]. *)
+      (*apply FlatPR_homomorphism_iff; eauto. *)
+    (*- destruct H as (H0 & H1).*)
+      (*split; [ apply A | split; [apply B | ]]. *)
+      (*apply FlatPR_homomorphism_iff in H1; eauto. *)
+  (*Qed. *)
+(*End fixInstance. *)
+
+
+(*Definition trivialNoInstance := Build_BinaryPR 0 0 [] [] [] 0. *)
+(*Lemma trivialNoInstance_isNoInstance : not (BinaryPRLang trivialNoInstance). *)
+(*Proof. *)
+  (*intros (H & _). destruct H as (H & _). cbn in H. lia. *)
+(*Qed. *)
+
+(*Definition reduction (fpr : FlatPR) := if FlatPR_wf_dec fpr && isValidFlattening_dec fpr && leb 1 (Sigma fpr) then hBinaryPR (h fpr) fpr else trivialNoInstance. *)
+
+(*Lemma reduction_correct (fpr : FlatPR) : FlatPRLang fpr <-> BinaryPRLang (reduction fpr).  *)
+(*Proof. *)
+  (*[>split; intros (H & H1). <]*)
+  (*[>- unfold reduction. rewrite (proj2 (FlatPR_wf_dec_correct _) H). <]*)
+    (*[>destruct (lt_dec 0 (Sigma fpr)). <]*)
+    (*[>+ <]*)
+    (*[>apply reduction_wf. <]*)
+(*Admitted. *)
