theories/L/Complexity/Cook/GenNP.v
@@ -11,10 +11,10 @@ Definition initialTapeForString (sig : finType) (s : list sig) :=
   end. 
 
 (*single-tape machine whose head will always start at the leftmost position (i.e. initial tapes are niltape or leftof) *)
-Definition GenNPflat : TM*nat*nat -> Prop:=
-  fun '(M,maxSize, steps (*in unary*)) =>
-    exists sig (M':mTM sig 1), isFlatteningTMOf M M' /\ (exists i, (exists f, loopM (initc M' ([|initialTapeForString i|])) steps = Some f)
-         /\ length i <= maxSize).
-
 Definition GenNP (i : { sig : finType & (mTM sig 1 * nat * nat)%type } ) : Prop := 
   match i with existT _ sig (tm, k, t) => exists inp, |inp| <= k /\ exists f, loopM (initc tm ([|initialTapeForString inp|])) t = Some f end. 
+
+Definition FlatGenNP : TM*nat*nat -> Prop:=
+  fun '(M,maxSize, steps (*in unary*)) =>
+    exists sig (M':mTM sig 1), isFlatteningTMOf M M' /\ GenNP (existT _ _ (M', maxSize, steps)). 
+
