theories/L/Complexity/Cook/PR_to_BinaryPR.v
@@ -1,4 +1,4 @@
-From PslBase Require Import Base FinTypes. 
+From PslBase Require Import Base FinTypes.
 From PslBase Require Import Vectors.Vectors. 
 From Undecidability.L.Complexity.Cook Require Import Prelim BinaryPR PR PR_homomorphisms. 
 Require Import Lia.
@@ -27,17 +27,6 @@ Section fixInstance.
     unfold hNat. destruct leb eqn:H. 
     - rewrite !app_length, !repEl_length. apply leb_complete in H. cbn. nia. 
     - now rewrite repEl_length.
-  Qed. 
-
-  Lemma repEl_app_inv (X : Type) (a : X) s1 s2 n : repEl n a = s1 ++ s2 -> exists n1 n2, s1 = repEl n1 a /\ s2 = repEl n2 a /\ n1 + n2 = n. 
-  Proof. 
-    revert s1 s2.  induction n. 
-    - cbn. destruct s1, s2; cbn; try congruence. intros _. exists 0, 0; now cbn.  
-    - cbn. destruct s1. 
-      + cbn. destruct s2; cbn; [ congruence | ]. 
-        intros H. inv H. exists 0, (S n); now cbn. 
-      + intros. cbn in H. inv H. apply IHn in H2 as (n1 & n2 & -> & -> & <-). 
-        exists (S n1), n2; now cbn. 
   Qed. 
 
   Lemma h'_inv1 (Sig x n : nat) : hNat Sig x = repEl n false ++ [true] ++ repEl (Sig - n -1) false -> x = n. 
@@ -78,8 +67,15 @@ Section fixInstance.
     now apply h'_inv1, injective_index in H. 
   Qed. 
 
-  Notation hoffset := (@hoffset (FinType (EqType bool)) pr h' h'_ge1 h'_uniform A1).
-  Notation hwidth := (@hwidth (FinType (EqType bool)) pr h' h'_ge1 h'_uniform A1). 
+  Lemma h'_length x : |h' x| = |elem Sigma|. 
+  Proof. 
+    unfold h'. now rewrite hNat_length.   
+  Qed. 
+
+  Definition h := h h'. 
+
+  Notation hoffset := (@hoffset pr (|elem Sigma|)).
+  Notation hwidth := (@hwidth pr (|elem Sigma|)). 
   Notation hinit := (@hinit (FinType (EqType bool)) pr h'). 
   Notation hwindows := (@hwindows (FinType (EqType bool)) pr h'). 
   Notation hfinal := (@hfinal (FinType (EqType bool)) pr h'). 
@@ -87,76 +83,40 @@ Section fixInstance.
 
   Definition hBinaryPR := @BinaryPR.Build_BinaryPR hoffset hwidth hinit hwindows hfinal hsteps. 
 
+  Lemma h_multiplier_sp x : |h x| = (|elem Sigma|) * |x|. 
+  Proof. 
+    unfold h. erewrite h_multiplier. 2: apply h'_length. easy.
+  Qed. 
+
   Lemma PR_homomorphism_wf : PR_wellformed pr -> BinaryPR.BinaryPR_wellformed hBinaryPR. 
   Proof. 
-    intros (H1 & H2 & H3 & H4 & H5 & H6). split; [ | split; [ | split]]; cbn. 
-    + unfold hwidth. specialize (@k_ge _ pr h' h'_ge1 h'_uniform A1). 
-      destruct A as (A2 & _). intros. remember (k h'_ge1 h'_uniform A1). setoid_rewrite <- Heqn. nia. 
-    + unfold hinit, hwidth. rewrite (h_multiplier h'_ge1 h'_uniform A1 init). 
-      remember (k h'_ge1 h'_uniform A1). setoid_rewrite <- Heqn. nia. 
+    intros (H1 & H2 & H3 & H4 & H5 & H6). 
+    unfold BinaryPR_wellformed; repeat match goal with [ |- _ /\ _] => split end; cbn. 
+    + unfold hwidth. nia. 
+    + unfold hoffset. nia. 
+    + unfold hwidth, hoffset. destruct H3 as (k' & H3 & H3'). exists k'. split; nia.  
+    + unfold hinit, hwidth. rewrite h_multiplier_sp. nia. 
     + unfold hwidth. intros [] H. unfold hwindows in H. apply in_map_iff in H as (win' & <- & H). 
       destruct win'. apply H5 in H. destruct H as (H & H0); cbn in *. 
-      split; cbn; now setoid_rewrite (h_multiplier h'_ge1 h'_uniform A1). 
+      split; cbn; now rewrite h_multiplier_sp. 
     + destruct H6 as (k' & H6). unfold hinit, hoffset. exists k'. 
-      rewrite (h_multiplier h'_ge1 h'_uniform A1 init), H6.
-      remember (k h'_ge1 h'_uniform A1). setoid_rewrite <- Heqn. nia. 
+      rewrite h_multiplier_sp, H6. nia. 
   Qed. 
 
   (*we now get the reduction for the case that the instance we reduce from is wellformed *)
   Lemma reduction_wf : PRLang pr <-> BinaryPRLang hBinaryPR. 
   Proof. 
-    (*specialize (h_bounded_injective) as F1. *)
-    (*specialize (h_uniform_homomorphism) as F2. *)
     split; intros. 
     - destruct H as (_ & sf & H1 & H2).
       split; [ apply PR_homomorphism_wf; auto | ]. 
       apply PR_homomorphism_iff; eauto. 
-      apply h'_injective. 
+      apply h'_injective. apply h'_length. 
     - destruct H as (_ & H1).
       split; [ apply A | ]. 
-      apply PR_homomorphism_iff in H1; eauto. apply h'_injective. 
+      apply (PR_homomorphism_iff h'_injective A1 A1 h'_length A) in H1. 
+      apply H1. 
   Qed. 
 End fixInstance. 
-
-Definition PRWin_of_size_dec (X : Type) width (win : PRWin X) := Nat.eqb (|prem win|) width && Nat.eqb (|conc win|) width.
-
-Lemma leb_iff a b : leb a b = true <-> a <= b. 
-Proof. 
-  split; intros. 
-  - now apply leb_complete. 
-  - now apply leb_correct. 
-Qed.
-
-Lemma PRWin_of_size_dec_correct (X : Type) width (win : PRWin X) : PRWin_of_size_dec width win = true <-> PRWin_of_size win width. 
-Proof. 
-  unfold PRWin_of_size, PRWin_of_size_dec. rewrite andb_true_iff. rewrite <- !(reflect_iff _ _ (Nat.eqb_spec _ _ )). easy.
-Qed. 
-
-Print PR_wellformed. 
-
-Definition PR_wf_dec (pr : PR) := 
-  leb 1 (width pr) 
-  && leb 1 (offset pr)
-  && Nat.eqb (Nat.modulo (width pr) (offset pr)) 0
-  && leb (width pr) (|init pr|)
-  && forallb (PRWin_of_size_dec (width pr)) (windows pr)
-  && Nat.eqb (Nat.modulo (|init pr|) (offset pr)) 0.
- 
-
-Lemma PR_wf_dec_correct (pr : PR) : PR_wf_dec pr = true <-> PR_wellformed pr. 
-Proof. 
-  unfold PR_wf_dec, PR_wellformed. rewrite !andb_true_iff, !and_assoc.
-  rewrite !leb_iff. rewrite <- !(reflect_iff _ _ (Nat.eqb_spec _ _ )).  
-  rewrite !forallb_forall. 
-  setoid_rewrite PRWin_of_size_dec_correct.  
-  split; intros; repeat match goal with [H : _ /\ _ |- _] => destruct H end; 
-  repeat match goal with [ |- _ /\ _ ] => split end; try easy. 
-  - apply Nat.mod_divide in H1 as (k & H1); [ | lia]. 
-    exists k; split; [ | apply H1 ]. destruct k; cbn in *; lia.
-  - apply Nat.mod_divide in H4 as (k & H4); [ | lia].  exists k; apply H4.  
-  - apply Nat.mod_divide; [ lia | ]. destruct H1 as (k & _ & H1). exists k; apply H1.
-  - apply Nat.mod_divide; [ lia | ]. apply H4. 
-Qed. 
 
 Definition trivialNoInstance := Build_BinaryPR 0 0 [] [] [] 0. 
 Lemma trivialNoInstance_isNoInstance : not (BinaryPRLang trivialNoInstance). 
@@ -164,16 +124,19 @@ Proof.
   intros (H & _). destruct H as (H & _). cbn in H. lia. 
 Qed. 
 
-Lemma reduction_correct (pr : PR) : { bpr & PRLang pr <-> BinaryPRLang bpr}.  
+Definition reduction (pr : PR) := if PR_wf_dec pr then hBinaryPR pr else trivialNoInstance. 
+
+Lemma PR_to_BinaryPR (pr : PR) : PRLang pr <-> BinaryPRLang (reduction pr).  
 Proof. 
+  unfold reduction. 
   destruct (PR_wf_dec pr) eqn:H1. 
   - apply PR_wf_dec_correct in H1. remember H1 as H0. clear HeqH0. destruct H1 as (H1 & _ & _ & H2 & _). 
-    destruct init; cbn in H2; [ exists trivialNoInstance; lia| ]. 
+    destruct init; cbn in H2; [ lia | ]. 
     assert (|elem (Sigma pr)| > 0). 
     { specialize (@elem_spec _ e). destruct elem; cbn; [eauto | lia]. }
-    exists (hBinaryPR H). apply reduction_wf, H0.   
+    apply reduction_wf; easy. 
   - assert (not (PR_wf_dec pr = true)) as H by eauto. rewrite PR_wf_dec_correct in H. 
-    exists trivialNoInstance. split; intros. 
+    split; intros. 
     + destruct H0; tauto. 
     + exfalso; apply trivialNoInstance_isNoInstance, H0. 
 Qed. 
