theories/L/Complexity/Cook/UniformHomomorphisms.v
@@ -1,0 +1,54 @@
+From PslBase Require Import Base FiniteTypes. 
+From Undecidability.L.Complexity.Cook Require Import Prelim.
+Require Import Lia.
+
+(*We define uniform homomorphisms (of strings): Given strings of the same length, they output strings of the same length.*)
+Section fixX.
+  Variable (X Y : Type). 
+
+  Definition homomorphism (h : list X -> list Y) := forall x1 x2, h (x1 ++ x2) = h x1 ++ h x2. 
+
+  Lemma homo_nil h : homomorphism h -> h [] = []. 
+  Proof. 
+    intros. unfold homomorphism in H. specialize (H [] []). 
+    cbn in H; rewrite H. destruct (h []) eqn:Heqn; cbn; [ congruence | ].  
+    assert (|y :: l| = |(y :: l) ++ y :: l|) as H0 by congruence. 
+    cbn in H0. rewrite app_length in H0. cbn in H0; lia. 
+  Qed. 
+
+  Lemma homo_cons h x l : homomorphism h -> h (x::l) = h [x] ++ h l.
+  Proof. 
+    intros. replace (x :: l) with ([x] ++ l) by now cbn. apply H. 
+  Qed.
+
+  Lemma homo_concat h : homomorphism h -> forall x, h (concat x) = concat (map h x). 
+  Proof. 
+    intros. induction x. 
+    - cbn. apply homo_nil, H. 
+    - cbn. rewrite H. now rewrite IHx. 
+  Qed. 
+
+  (*the last condition excludes the trivial homomorphism x ↦ ε *)
+  Definition uniform_homomorphism (h : list X -> list Y) := homomorphism h /\ (forall x y, |h [x]| = |h [y]|) /\ (forall x, |h[x]| >= 1).
+
+  Lemma unif_homo_length h x y : uniform_homomorphism h -> |x| = |y| -> |h x| = |h y|. 
+  Proof. 
+    intros (H1 & H2 & _). 
+    revert y. induction x; intros. 
+    - destruct y; cbn in *; [ | congruence]. now cbn. 
+    - destruct y; cbn in *; [ congruence | ]. 
+      replace (a :: x) with ([a] ++ x) by now cbn. replace (x0 :: y) with ([x0] ++ y) by now cbn. 
+      rewrite !H1. rewrite !app_length. erewrite H2 with (y := x0). 
+      rewrite IHx with (y := y); eauto. 
+  Qed. 
+
+  (*given an arbitrary function mapping elements of X into strings over Y, we can derive a homomorphism *)
+  Definition canonicalHom (h' : X -> list Y) := fun (l : list X) => concat (map h' l). 
+  Lemma canonicalHom_is_homomorphism h' : homomorphism (canonicalHom h'). 
+  Proof. 
+    unfold homomorphism. intros. unfold canonicalHom. 
+    now rewrite map_app, concat_app. 
+  Qed. 
+End fixX. 
+
+
